The given equation is a cubic equation of the form ax^3 + bx^2 + cx + d = 0, where a = 1, b = -4, c = 6, and d = -24. To solve this equation, we can use the following steps:

1. Factor the equation: x^3 - 4x^2 + 6x - 24 = 0
2. Find the roots of the equation by factoring: (x - 4)(x^2 - x - 6) = 0
3. Solve the quadratic equation: x^2 - x - 6 = 0
4. Use the quadratic formula to find the roots of the quadratic equation: x = (1 ± √(1^2 - 4(1)(-6)))/(2(1)) = (1 ± √(25))/2 = (1 ± 5)/2
5. The roots of the cubic equation are: x = 4, x = (1 + √25)/2 = 3, and x = (1 - √25)/2 = -2

Therefore, the solutions to the given equation are: x = 4, x = 3, and x = -2.