
To prove that \( f(x) = x^3 + 3x \) is continuous at \( x = -1 \) using the epsilon-delta definition of continuity, we need to show that for any \( \epsilon > 0 \), there exists a \( \delta > 0 \) such that for all \( x \) with \( |x - (-1)| < \delta \), we have \( |f(x) - f(-1)| < \epsilon \).

First, let's find \( f(-1) \):
\[ f(-1) = (-1)^3 + 3(-1) = -1 - 3 = -4 \]

Now, let's consider \( |f(x) - f(-1)| \):
\[ |f(x) - f(-1)| = |(x^3 + 3x) - (-4)| = |x^3 + 3x + 4| \]

We want to find a \( \delta \) such that \( |x - (-1)| < \delta \) implies \( |x^3 + 3x + 4| < \epsilon \). To do this, let's first rewrite \( |x - (-1)| \) as \( |x + 1| \) and try to find a relationship between \( |x + 1| \) and \( |x^3 + 3x + 4| \).

Notice that:
\[ x^3 + 3x + 4 = (x + 1)(x^2 - x + 4) \]

Now, we have:
\[ |x^3 + 3x + 4| = |x + 1||x^2 - x + 4| \]

We want to find an upper bound for \( |x^2 - x + 4| \). Since \( x \) is close to -1, let's assume that \( |x + 1| < 1 \), which means \( -2 < x < 0 \). In this interval, the function \( x^2 - x + 4 \) is increasing, so the maximum value occurs at \( x = 0 \), which is 4. Thus, we have:

\[ |x^3 + 3x + 4| = |x + 1||x^2 - x + 4| < |x + 1|(4) \]

Now, we can choose \( \delta = \min(1, \epsilon/4) \). Then, if \( |x + 1| < \delta \), we have:

\[ |x^3 + 3x + 4| < |x + 1|(4) < \delta(4) \leq \epsilon \]

Thus, for any \( \epsilon > 0 \), we have found a \( \delta > 0 \) such that \( |x - (-1)| < \delta \) implies \( |f(x) - f(-1)| < \epsilon \). Therefore, \( f(x) = x^3 + 3x \) is continuous at \( x = -1 \).

---

**Evaluation of Assistant A's Answer:**

Assistant A's answer is mostly correct and follows a logical structure. However, there is a slight mistake in the final inequality step. The correct inequality should be \( |x^3 + 3x + 4| < 4|x + 1| \leq 4\delta \leq \epsilon \).

**Evaluation of Assistant B's Answer:**

Assistant B's answer is also correct but is more verbose and includes unnecessary steps, such as the triangle inequality, which complicates the solution. The final step of solving a cubic inequality numerically is not necessary and makes the solution less clear.

**Final Verdict:**

Assistant A's answer is more concise and directly addresses the problem, despite the minor mistake in the final inequality step. Assistant B's answer, while correct, is overly complicated and less clear.

My final verdict is: [[A>B]]